basic flatMap

src/Init/Data/Iterators/Combinators/Monadic/FlatMap.lean
@@ -9,10 +9,12 @@ prelude
 public import Init.Data.Iterators.Basic
 public import Init.Data.Iterators.Consumers.Collect
 public import Init.Data.Iterators.Consumers.Loop
+public import Init.Data.Iterators.Combinators.Monadic.FilterMap
 public import Init.Data.Iterators.PostconditionMonad
 public import Init.Data.Iterators.Internal.Termination
+public import Init.Data.Option.Lemmas
 
-public section
+public import Std.Data.Iterators.Producers.List
 
 set_option doc.verso true
 
@@ -33,12 +35,207 @@ Several variants of `flatMap` are provided:
 
 namespace Std.Iterators
 
-@[unbox]
-structure FlatMap (α : Type w) [Iterator α m β]
-    (f : (it : IterM (α := α) m β) → (out : β) → it.IsPlausibleOutput out → IterM (α := α₂) m γ) where
-  it₁ : IterM (α := α) m β
-  it₂ : Option (IterM (α := α₂) m γ)
+@[ext, unbox]
+public structure Flatten (α α₂ β : Type w) (m) where
+  it₁ : IterM (α := α) m (IterM (α := α₂) m β)
+  it₂ : Option (IterM (α := α₂) m β)
 
+@[always_inline]
+def IterM.flattenAfter {α α₂ β : Type w} {m : Type w → Type w'} [Monad m]
+    [Iterator α m (IterM (α := α₂) m β)] [Iterator α₂ m β]
+    (it₁ : IterM (α := α) m (IterM (α := α₂) m β)) (it₂ : Option (IterM (α := α₂) m β)) :=
+  (toIterM (α := Flatten α α₂ β m) ⟨it₁, it₂⟩ m β : IterM m β)
 
+@[always_inline]
+public def IterM.flatMapAfter {α : Type w} {β : Type w} {α₂ : Type w}
+    {γ : Type w} {m : Type w → Type w'} [Monad m] [Iterator α m β] [Iterator α₂ m γ]
+    (f : β → IterM (α := α₂) m γ) (it₁ : IterM (α := α) m β) (it₂ : Option (IterM (α := α₂) m γ)) :=
+  ((it₁.map f).flattenAfter it₂ : IterM m γ)
+
+@[always_inline]
+public def IterM.flatMap {α : Type w} {β : Type w} {α₂ : Type w}
+    {γ : Type w} {m : Type w → Type w'} [Monad m] [Iterator α m β] [Iterator α₂ m γ]
+    (f : β → IterM (α := α₂) m γ) (it : IterM (α := α) m β) :=
+  (it.flatMapAfter f none : IterM m γ)
+
+variable {α α₂ β : Type w} {m : Type w → Type w'}
+
+public inductive Flatten.IsPlausibleStep [Iterator α m (IterM (α := α₂) m β)] [Iterator α₂ m β] :
+    (it : IterM (α := Flatten α α₂ β m) m β) → (step : IterStep (IterM (α := Flatten α α₂ β m) m β) β) → Prop where
+  | outerYield : ∀ {it₁ it₁' it₂'}, it₁.IsPlausibleStep (.yield it₁' it₂') →
+      IsPlausibleStep (toIterM ⟨it₁, none⟩ m β) (.skip (toIterM ⟨it₁', some it₂'⟩ m β))
+  | outerSkip : ∀ {it₁ it₁'}, it₁.IsPlausibleStep (.skip it₁') →
+      IsPlausibleStep (toIterM ⟨it₁, none⟩ m β) (.skip (toIterM ⟨it₁', none⟩ m β))
+  | outerDone : ∀ {it₁}, it₁.IsPlausibleStep .done →
+      IsPlausibleStep (toIterM ⟨it₁, none⟩ m β) .done
+  | innerYield : ∀ {it₁ it₂ it₂' b}, it₂.IsPlausibleStep (.yield it₂' b) →
+      IsPlausibleStep (toIterM ⟨it₁, some it₂⟩ m β) (.yield (toIterM ⟨it₁, some it₂'⟩ m β) b)
+  | innerSkip : ∀ {it₁ it₂ it₂'}, it₂.IsPlausibleStep (.skip it₂') →
+      IsPlausibleStep (toIterM ⟨it₁, some it₂⟩ m β) (.skip (toIterM ⟨it₁, some it₂'⟩ m β))
+  | innerDone : ∀ {it₁ it₂}, it₂.IsPlausibleStep .done →
+      IsPlausibleStep (toIterM ⟨it₁, some it₂⟩ m β) (.skip (toIterM ⟨it₁, none⟩ m β))
+
+public instance Flatten.instIterator [Monad m] [Iterator α m (IterM (α := α₂) m β)] [Iterator α₂ m β] :
+    Iterator (Flatten α α₂ β m) m β where
+  IsPlausibleStep := IsPlausibleStep
+  step it :=
+    match it with
+    | ⟨it₁, none⟩ => do
+      match ← it₁.step with
+      | .yield it₁' it₂' h =>
+          pure <| .skip ⟨it₁', some it₂'⟩ (.outerYield h)
+      | .skip it₁' h =>
+          pure <| .skip ⟨it₁', none⟩ (.outerSkip h)
+      | .done h =>
+          pure <| .done (.outerDone h)
+    | ⟨it₁, some it₂⟩ => do
+      match ← it₂.step with
+      | .yield it₂' c h =>
+          pure <| .yield ⟨it₁, some it₂'⟩ c (.innerYield h)
+      | .skip it₂' h =>
+          pure <| .skip ⟨it₁, some it₂'⟩ (.innerSkip h)
+      | .done h =>
+          pure <| .skip ⟨it₁, none⟩ (.innerDone h)
+
+section Finite
+
+variable {α : Type w} {α₂ : Type w} {β : Type w} {m : Type w → Type w'}
+
+variable (α m β) in
+def Rel [Monad m] [Iterator α m (IterM (α := α₂) m β)] [Iterator α₂ m β] [Finite α m] [Finite α₂ m] :
+    IterM (α := Flatten α α₂ β m) m β → IterM (α := Flatten α α₂ β m) m β → Prop :=
+  InvImage
+    (Prod.Lex
+      (InvImage IterM.TerminationMeasures.Finite.Rel IterM.finitelyManySteps)
+      (Option.lt (InvImage IterM.TerminationMeasures.Finite.Rel IterM.finitelyManySteps)))
+    (fun it => (it.internalState.it₁, it.internalState.it₂))
+
+theorem Flatten.rel_of_left [Monad m] [Iterator α m (IterM (α := α₂) m β)] [Iterator α₂ m β]
+    [Finite α m] [Finite α₂ m] {it it'}
+    (h : it'.internalState.it₁.finitelyManySteps.Rel it.internalState.it₁.finitelyManySteps) :
+    Rel α β m it' it :=
+  Prod.Lex.left _ _ h
+
+theorem Flatten.rel_of_right₁ [Monad m] [Iterator α m (IterM (α := α₂) m β)] [Iterator α₂ m β]
+    [Finite α m] [Finite α₂ m] {it₁ it₂ it₂'}
+    (h : (InvImage IterM.TerminationMeasures.Finite.Rel IterM.finitelyManySteps) it₂' it₂) :
+    Rel α β m ⟨it₁, some it₂'⟩ ⟨it₁, some it₂⟩ := by
+  refine Prod.Lex.right _ h
+
+theorem Flatten.rel_of_right₂ [Monad m] [Iterator α m (IterM (α := α₂) m β)] [Iterator α₂ m β]
+    [Finite α m] [Finite α₂ m] {it₁ it₂} :
+    Rel α β m ⟨it₁, none⟩ ⟨it₁, some it₂⟩ :=
+  Prod.Lex.right _ True.intro
+
+instance [Monad m] [Iterator α m (IterM (α := α₂) m β)] [Iterator α₂ m β]
+    [Finite α m] [Finite α₂ m] :
+    FinitenessRelation (Flatten α α₂ β m) m where
+  rel := Rel α β m
+  wf := by
+    apply InvImage.wf
+    refine ⟨fun (a, b) => Prod.lexAccessible (WellFounded.apply ?_ a) (WellFounded.apply ?_) b⟩
+    · exact InvImage.wf _ WellFoundedRelation.wf
+    · exact Option.wellFounded_lt <| InvImage.wf _ WellFoundedRelation.wf
+  subrelation {it it'} h := by
+    obtain ⟨step, h, h'⟩ := h
+    cases h' <;> cases h
+    case outerYield =>
+      apply Flatten.rel_of_left
+      exact IterM.TerminationMeasures.Finite.rel_of_yield ‹_›
+    case outerSkip =>
+      apply Flatten.rel_of_left
+      exact IterM.TerminationMeasures.Finite.rel_of_skip ‹_›
+    case innerYield =>
+      apply Flatten.rel_of_right₁
+      exact IterM.TerminationMeasures.Finite.rel_of_yield ‹_›
+    case innerSkip =>
+      apply Flatten.rel_of_right₁
+      exact IterM.TerminationMeasures.Finite.rel_of_skip ‹_›
+    case innerDone =>
+      apply Flatten.rel_of_right₂
+
+@[no_expose]
+public instance [Monad m] [Iterator α m (IterM (α := α₂) m β)] [Iterator α₂ m β]
+    [Finite α m] [Finite α₂ m] : Finite (Flatten α α₂ β m) m :=
+  .of_finitenessRelation instFinitenessRelationFlattenOfIterMOfFinite
+
+end Finite
+
+section Productive
+
+variable {α : Type w} {α₂ : Type w} {β : Type w} {m : Type w → Type w'}
+
+variable (α m β) in
+def ProductiveRel [Monad m] [Iterator α m (IterM (α := α₂) m β)] [Iterator α₂ m β] [Finite α m]
+    [Productive α₂ m] :
+    IterM (α := Flatten α α₂ β m) m β → IterM (α := Flatten α α₂ β m) m β → Prop :=
+  InvImage
+    (Prod.Lex
+      (InvImage IterM.TerminationMeasures.Finite.Rel IterM.finitelyManySteps)
+      (Option.lt (InvImage IterM.TerminationMeasures.Productive.Rel IterM.finitelyManySkips)))
+    (fun it => (it.internalState.it₁, it.internalState.it₂))
+
+theorem Flatten.productiveRel_of_left [Monad m] [Iterator α m (IterM (α := α₂) m β)]
+    [Iterator α₂ m β] [Finite α m] [Productive α₂ m] {it it'}
+    (h : it'.internalState.it₁.finitelyManySteps.Rel it.internalState.it₁.finitelyManySteps) :
+    ProductiveRel α β m it' it :=
+  Prod.Lex.left _ _ h
+
+theorem Flatten.productiveRel_of_right₁ [Monad m] [Iterator α m (IterM (α := α₂) m β)] [Iterator α₂ m β]
+    [Finite α m] [Productive α₂ m] {it₁ it₂ it₂'}
+    (h : (InvImage IterM.TerminationMeasures.Productive.Rel IterM.finitelyManySkips) it₂' it₂) :
+    ProductiveRel α β m ⟨it₁, some it₂'⟩ ⟨it₁, some it₂⟩ := by
+  refine Prod.Lex.right _ h
+
+theorem Flatten.productiveRel_of_right₂ [Monad m] [Iterator α m (IterM (α := α₂) m β)] [Iterator α₂ m β]
+    [Finite α m] [Productive α₂ m] {it₁ it₂} :
+    ProductiveRel α β m ⟨it₁, none⟩ ⟨it₁, some it₂⟩ :=
+  Prod.Lex.right _ True.intro
+
+instance [Monad m] [Iterator α m (IterM (α := α₂) m β)] [Iterator α₂ m β]
+    [Finite α m] [Productive α₂ m] :
+    ProductivenessRelation (Flatten α α₂ β m) m where
+  rel := ProductiveRel α β m
+  wf := by
+    apply InvImage.wf
+    refine ⟨fun (a, b) => Prod.lexAccessible (WellFounded.apply ?_ a) (WellFounded.apply ?_) b⟩
+    · exact InvImage.wf _ WellFoundedRelation.wf
+    · exact Option.wellFounded_lt <| InvImage.wf _ WellFoundedRelation.wf
+  subrelation {it it'} h := by
+    cases h
+    case outerYield =>
+      apply Flatten.productiveRel_of_left
+      exact IterM.TerminationMeasures.Finite.rel_of_yield ‹_›
+    case outerSkip =>
+      apply Flatten.productiveRel_of_left
+      exact IterM.TerminationMeasures.Finite.rel_of_skip ‹_›
+    case innerSkip =>
+      apply Flatten.productiveRel_of_right₁
+      exact IterM.TerminationMeasures.Productive.rel_of_skip ‹_›
+    case innerDone =>
+      apply Flatten.productiveRel_of_right₂
+
+@[no_expose]
+public instance [Monad m] [Iterator α m (IterM (α := α₂) m β)] [Iterator α₂ m β]
+    [Finite α m] [Productive α₂ m] : Productive (Flatten α α₂ β m) m :=
+  .of_productivenessRelation instProductivenessRelationFlattenOfFiniteIterMOfProductive
+
+end Productive
+
+public instance Flatten.instIteratorCollect [Monad m] [Monad n] [Iterator α m (IterM (α := α₂) m β)]
+    [Iterator α₂ m β] : IteratorCollect (Flatten α α₂ β m) m n :=
+  .defaultImplementation
+
+public instance Flatten.instIteratorCollectPartial [Monad m] [Monad n] [Iterator α m (IterM (α := α₂) m β)]
+    [Iterator α₂ m β] : IteratorCollectPartial (Flatten α α₂ β m) m n :=
+  .defaultImplementation
+
+public instance Flatten.instIteratorLoop [Monad m] [Monad n] [Iterator α m (IterM (α := α₂) m β)]
+    [Iterator α₂ m β] : IteratorLoop (Flatten α α₂ β m) m n :=
+  .defaultImplementation
+
+public instance Flatten.instIteratorLoopPartial [Monad m] [Monad n] [Iterator α m (IterM (α := α₂) m β)]
+    [Iterator α₂ m β] : IteratorLoopPartial (Flatten α α₂ β m) m n :=
+  .defaultImplementation
 
 end Std.Iterators
